relational semantics of existential types with difunctional closure

coq/Rel.v
@@ -5,6 +5,7 @@ Import Coq.Init.Notations.
 
 Require Export Coq.Classes.Morphisms.
 Require Export Relations.
+Require Import Casts.
 
 Section RelDefs.
   Variable A B:Type.
@@ -12,6 +13,21 @@ Section RelDefs.
   Variable S:relation B.
 
   Definition difunctional := forall x x' y y', R x y -> R x' y' -> R x y' -> R x' y.
+
+  Inductive difclo : A -> A -> Prop :=
+  | difclo_base : forall x y,
+                    R x y ->
+                    difclo x y
+  | difclo_step : forall x x' y y',
+                    difclo x y ->
+                    difclo x' y' ->
+                    difclo x y' ->
+                    difclo x' y.
+
+  Definition PER :=
+    (forall x y, R x y -> R y x)
+      /\
+      (forall x y z, R x y -> R y z -> R x z).
 
   (* Relation constructions *)
   Definition RelId    := (fun x y => x=y) : relation A.
@@ -27,6 +43,7 @@ Section RelDefs.
 
   (* Composition and inversion *)
   Definition RelComp := (fun x y => exists z, R x z /\ R' z y) : relation A.
+  Definition RelInv  := (fun x y => R y x) : relation A.
 
   (* Relation equality *)
   Definition RelEq := forall x y, R x y <-> R' x y.
@@ -35,7 +52,10 @@ End RelDefs.
 
 Implicit Arguments RelId [].
 Implicit Arguments difunctional. 
+Implicit Arguments difclo.
+Implicit Arguments PER.
 Implicit Arguments RelComp [A]. 
+Implicit Arguments RelInv [A].
 Implicit Arguments RelArrow.
 Implicit Arguments RelProd. 
 Implicit Arguments RelSum. 
@@ -125,5 +145,166 @@ Section RelLemmas.
     eauto.
   Qed.
 
-End RelLemmas.    
+  Lemma difclo_difunctional : difunctional (difclo R).
+  Proof.
+    unfold difunctional. apply difclo_step.
+  Qed.
 
+  Lemma difclo_monotonic : 
+    forall R' : relation A,
+      (forall x y, R x y -> R' x y) ->
+      forall x y,
+        difclo R x y -> difclo R' x y. 
+  Proof.
+    intros R' incl x y difclo_R_x_y.
+    induction difclo_R_x_y.
+    (* base *)
+      apply difclo_base. apply incl. assumption.
+    (* step *)
+      eapply difclo_step; eassumption.
+  Qed.
+
+  Lemma difclo_inv :
+    (forall x y, R x y -> R y x) ->
+    (forall x y, difclo R x y -> difclo R y x).
+  Proof.
+    intros R_inv x y difclo_R_x_y.
+    induction difclo_R_x_y.
+     (* base *) apply difclo_base. intuition.
+     (* step *) eapply difclo_step; eassumption.
+  Qed.
+
+  Lemma difclo_closure : difunctional R -> RelEq R (difclo R).
+  Proof.
+    intros dif. unfold RelEq. intros x y. split.
+    (* -> *)
+      intros r. apply difclo_base. assumption.
+    (* <- *)
+      intros dif_r. induction dif_r.
+      (* difclo_base *)
+        assumption.
+      (* difclo_step *)
+        unfold difunctional in dif.
+        eapply dif; eassumption.
+  Qed.
+
+  Lemma difclo_ext : forall R', RelEq R R' -> RelEq (difclo R) (difclo R').
+  Proof.
+    intros R' R_eq_R'.
+    intros x y. split.
+    (* -> *)
+      intro difclo_R_x_y. induction difclo_R_x_y. 
+       apply difclo_base. apply R_eq_R'. assumption.
+       eapply difclo_step; eassumption.
+    (* <- *)
+      intro difclo_R'_x_y. induction difclo_R'_x_y. 
+       apply difclo_base. apply R_eq_R'. assumption.
+       eapply difclo_step; eassumption.
+  Qed.
+
+  Lemma difclo_cast :
+    forall (C D : Type) (R1 : relation C) (R2 : relation D) (eq : C = D),
+      (forall x y, R1 x y -> R2 (x :? eq) (y :? eq)) ->
+      forall x y, difclo R1 x y -> difclo R2 (x :? eq) (y :? eq).
+  Proof.
+    intros C D R1 R2 eq R1_R2 x y difclo_R_x_y.
+    induction difclo_R_x_y.
+    (* base *)
+      apply difclo_base. apply R1_R2. assumption.
+    (* step *)
+      eapply difclo_step; eassumption.
+  Qed.
+
+  Lemma difclo_cast2 : 
+    forall (C D : Type) (R1 : relation C) (R2 : relation D) (eq : D = C),
+      (forall x y, R1 (x :? eq) (y :? eq) -> R2 x y) ->
+      forall x y, difclo R1 (x :? eq) (y :? eq) -> difclo R2 x y.
+  Proof.
+    intros C D R1 R2 eq R1_R2 x y.
+    replace x with ((x :? eq) :? sym_equal eq).
+    replace y with ((y :? eq) :? sym_equal eq).
+    intro. apply difclo_cast with (R1:=R1).
+     intros x' y' r. apply (R1_R2 (x' :? sym_equal eq) (y' :? sym_equal eq)).
+       rewrite cast_coalesce. rewrite cast_id.
+       rewrite cast_coalesce. rewrite cast_id.
+       assumption.
+    rewrite cast_coalesce in H. rewrite cast_id in H.
+    rewrite cast_coalesce in H. rewrite cast_id in H.
+    assumption.
+    rewrite cast_coalesce. apply cast_id.
+    rewrite cast_coalesce. apply cast_id.
+  Qed.
+
+  Lemma difclo_cast3 : 
+    forall (R' : relation B) (eq : B = A),
+      (forall x y, R (x :? eq) (y :? eq) <-> R' x y) ->
+      forall x y, difclo R (x :? eq) (y :? eq) <-> difclo R' x y.
+  Proof.
+    intros R' eq R_R' x y. split.
+    apply difclo_cast2. apply R_R'.
+    apply difclo_cast. apply R_R'.
+  Qed.
+
+  (* Difunctional relations and PERs *)
+
+  Lemma difunctional_yields_per_left :
+    difunctional R ->
+    PER (R o (RelInv R)).
+  Proof.
+    intro DIF. unfold RelComp. unfold RelInv. split. 
+    (* symmetric *)
+    intros x y [z [R1 R2]]. exists z. auto.
+    (* transitive *)
+    intros x y z [z1 [R1 R2]] [z2 [R3 R4]].
+    exists z1. split.
+      assumption.
+      eapply DIF; eassumption.
+  Qed.
+
+  Lemma difunctional_yields_per_right :
+    difunctional R ->
+    PER ((RelInv R) o R).
+  Proof.
+    intro DIF. unfold RelComp. unfold RelInv. split. 
+    (* symmetric *)
+    intros x y [z [R1 R2]]. exists z. auto.
+    (* transitive *)
+    intros x y z [z1 [R1 R2]] [z2 [R3 R4]].
+    exists z1. split.
+      assumption.
+      eapply DIF; eassumption.
+  Qed.
+
+  Definition Saturated R1 R2 :=
+    forall x1 x2 x3 x4,
+      R1 x1 x2 -> R x2 x3 -> R2 x3 x4 -> R x1 x4.
+
+  (* If 'R' is a QPER, then it is a saturated relation between the two PERS derived *)
+  Lemma qper_saturated :
+    difunctional R ->
+    Saturated (difclo R o RelInv (difclo R)) (RelInv (difclo R) o difclo R).
+  Proof.
+    intro DIF.
+    unfold Saturated. unfold RelComp. unfold RelInv.
+    intros x1 x2 x3 x4 [z1 [R1 R2]] R3 [z2 [R4 R5]].
+    apply difclo_closure. apply DIF.
+    assert (difclo R x2 x3). apply difclo_closure; assumption.
+    eauto using difclo_difunctional.
+  Qed.
+
+  Lemma reflexive_qper_transitive :
+    (forall x, R x x) ->
+    difunctional R ->
+    (forall x y z, R x y -> R y z -> R x z).
+  Proof.
+    intros REFL DIF. intros x y z R1 R2.
+    eapply DIF. apply R2. apply R1. apply REFL.
+  Qed.
+
+  Lemma functionalrel_difunctional :
+    forall (f : A -> A), difunctional (fun x y => f x = y).
+  Proof.
+    intro f. unfold difunctional. congruence.
+  Qed.
+
+End RelLemmas.
