coq/sem-difclo.v
@@ -1,0 +1,705 @@
+Require Import ssreflect ssrbool ssrfun seq.
+Require Import Relations Program.Equality.
+Require Import FunctionalExtensionality. 
+Set Implicit Arguments.
+Unset Strict Implicit.
+Import Prenex Implicits.
+
+Require Import syn Casts.
+
+Reserved Notation "| t |" (at level 60).
+
+(*---------------------------------------------------------------------------
+   Underlying semantics
+   ---------------------------------------------------------------------------*)
+Section Sem.
+
+Variable sig: SIG.
+Variable interpPrim: PrimType sig -> Type.
+
+(* Index-erasure interpretation of types, parameterized
+   on the interpretation of primitive types *)
+Fixpoint interpTy D (t: Ty D) : Type :=
+  match t with
+  | TyUnit       => unit
+  | TyProd t1 t2 => |t1| * |t2|
+  | TySum  t1 t2 => |t1| + |t2|
+  | TyArr  t1 t2 => |t1| -> |t2|
+  | TyAll    _ t => |t| 
+  | TyExists _ t => |t|
+  | TyPrim   p _ => interpPrim p
+  end%type
+where "| t |" := (interpTy t).
+
+Fixpoint existentialFree D (t: Ty (sig:=sig) D) :=
+  match t with
+  | TyUnit       => True
+  | TyProd t1 t2 => existentialFree t1 /\ existentialFree t2
+  | TySum  t1 t2 => existentialFree t1 /\ existentialFree t2
+  | TyArr  t1 t2 => existentialFree t1 /\ existentialFree t2
+  | TyAll    _ t => existentialFree t
+  | TyExists _ t => False
+  | TyPrim   p _ => True
+  end.
+
+Fixpoint interpCtxt D (G: Ctxt D) : Type :=
+  if G is t::G then (interpTy t * interpCtxt G)%type else unit.
+
+(* This is lemma 3, part 1 *)
+Lemma interpEquiv D (t1 t2: Ty D) A : equivTy A t1 t2 -> |t1| = |t2|.
+Proof. move => E. induction E => /=//; congruence. Qed. 
+
+(* This is lemma 3, part 2 *)
+Lemma interpSubst D (t: Ty D) : forall D' (S: Sub D D'), |t| = |apSubTy S t|.
+Proof. induction t => /=//; congruence. Qed.
+
+Lemma interpTyAll D s (t: Ty (s::D)) e : |TyAll t| = |apSubTy (consSub e (idSub D)) t|.
+Proof. by rewrite -interpSubst. Qed.
+
+Lemma interpTyExists D s (t: Ty (s::D)) e : |apSubTy (consSub e (idSub D)) t| = |TyExists t|.
+Proof. by rewrite -interpSubst. Qed.
+
+Lemma interpTyPack D s (t: Ty (s::D)) : |TyExists t| = |t|. Proof. done. Qed.
+
+Lemma interpSubCtxt D (G: Ctxt D) : forall D' (S: Sub D D'), interpCtxt G = interpCtxt (apSubCtxt S G). 
+Proof. 
+induction G. done. move => D' S. simpl. by rewrite (interpSubst t S) (IHG _ S). 
+Qed. 
+
+Fixpoint interpTmVar D (G: Ctxt D) (t: Ty D) (v: TmVar G t) : interpCtxt G -> (|t|) :=
+  match v with
+  | TmVarZ _ _ => fun eta => eta.1
+  | TmVarS _ _ _ v => fun eta => interpTmVar v eta.2
+  end.
+
+Variable A: seq (Ax sig). 
+
+Fixpoint interpTm D (G: Ctxt D) (t: Ty D) (M: Tm A G t) : interpCtxt G -> (|t|) :=
+  match M in Tm _ _ t return interpCtxt G -> |t| with
+  | VAR _ v       => fun eta => interpTmVar v eta
+  | UNIT          => fun eta => tt
+  | TYEQ _ _ pf M => fun eta => interpTm M eta :? interpEquiv pf 
+  | PAIR _ _ M N  => fun eta => (interpTm M eta, interpTm N eta)
+  | PROJ1 _ _ M   => fun eta => (interpTm M eta).1
+  | PROJ2 _ _ M   => fun eta => (interpTm M eta).2
+  | INL _ _ M     => fun eta => inl _ (interpTm M eta)
+  | INR _ _ M     => fun eta => inr _ (interpTm M eta)
+  | CASE _ _ _ M M1 M2 => fun eta => 
+    match interpTm M eta with 
+    | inl x => interpTm M1 (x,eta) 
+    | inr y => interpTm M2 (y,eta) 
+    end
+  | ABS _ _ M     => fun eta => fun x => interpTm M (x,eta)
+  | APP _ _ M N   => fun eta => (interpTm M eta) (interpTm N eta)
+  | UNIVABS s t M  => fun eta => interpTm M (eta :? interpSubCtxt G (pi D s))
+  | UNIVAPP s t e M => fun eta => interpTm M eta :? interpTyAll t e
+  | EXPACK _ e t M => fun eta => interpTm M eta :? interpTyExists t e
+  | EXUNPACK s t t' M N => fun eta => 
+    interpTm N (interpTm M eta :? interpTyPack t, eta :? interpSubCtxt G (pi D s)) 
+      :? sym_equal (interpSubst t' (pi D s))
+  end.
+
+(*---------------------------------------------------------------------------
+   Relational semantics
+
+   Some problems with logical relations:
+   * Existentials mess up proof that difunctional environments => difunctional semantics
+   * Would like to prove composition property but function types mess it up
+   * Perhaps should attempt to use prelogical relations of some kind
+   * Or perhaps we could do perp-perp for existentials
+   * Or perhaps just take "difunctional closure"
+   ---------------------------------------------------------------------------*)
+
+(* Relation environments *)
+Definition RelEnv D := 
+  forall p, Sub (tyArity p) D -> relation (interpPrim p).
+
+Require Import Rel.
+Definition invEnv D (R: RelEnv D) : RelEnv D := fun p ixs => fun x y => R p ixs y x.
+Definition composeEnv D (R1 R2: RelEnv D) : RelEnv D := 
+  fun p ixs => RelComp (R1 p ixs) (R2 p ixs).
+
+
+(* Relation environments that respect equivalence for a set of axioms A *)
+Definition GoodRelEnv D A (rho: RelEnv D) :=
+  forall p ixs ixs', equivSeq A ixs ixs' -> rho p (expsAsSub ixs) = rho p (expsAsSub ixs'). 
+
+(* Compose environment with substitution *)
+Definition EcS D D' (rho: RelEnv D') (S: Sub D D') : RelEnv D
+:= fun p S' => rho p (ScS S S').
+
+(* rho' extends rho on a variable of sort s *)
+Definition ext D (rho: RelEnv D) s (rho': RelEnv (s::D)) := EcS rho' (pi _ s) = rho.
+Notation "rho' >> rho" := (ext rho rho') (at level 70). 
+
+(* This is \cal E from Section 4.2.2 *)
+Definition RelEnvSet := forall D, RelEnv D -> Prop.
+
+Notation "'forall:' x 'in' S ',' P" := (forall x, S x -> P) 
+  (at level 200, x ident, right associativity) : type_scope.
+Notation "'exists:' x 'in' S ',' P" := (exists x, S x /\ P) 
+  (at level 200, x ident, right associativity) : type_scope.
+
+
+(* These are the two conditions on sets of environments specified in 4.2.2 *)
+(* We also include the condition that environments respect equivalence *)
+Structure ClosedRelEnvSet A (E:RelEnvSet) := {
+  goodEnvs : forall D rho, E D rho -> GoodRelEnv A rho;
+  closedWrtSubst : forall D D' (S: Sub D' D) rho, E D rho -> E D' (EcS rho S);
+  closedWrtInv : forall D rho, E D rho -> E D (invEnv rho);
+  closedWrtCompose : forall D rho1 rho2, E D rho1 -> E D rho2 -> E D (composeEnv rho1 rho2);
+  closedWrtLift : forall D D' s (S: Sub D' D), 
+  forall: rho1 in E (s::D'),
+  forall: rho2 in E D,
+  rho1 >> EcS rho2 S ->
+  exists: rho in E (s::D), 
+  EcS rho (liftSub s S) = rho1 /\
+  rho >> rho2
+}.
+
+Variable ES: RelEnvSet. 
+
+Fixpoint semTy D (rho: RelEnv D) (t:Ty D) : relation (|t|) :=
+  match t return relation (|t|) with
+  | TyUnit       => fun x y => True
+  | TyProd t1 t2 => fun x y => semTy rho x.1 y.1 /\ semTy rho x.2 y.2
+  | TySum t1 t2  => fun x y => 
+    match x, y with inl x1, inl y1 => semTy rho x1 y1
+                  | inr x2, inr y2 => semTy rho x2 y2
+                  | _, _ => False 
+    end
+  | TyArr t1 t2  => fun x y => forall x' y', semTy rho x' y' -> semTy rho (x x') (y y')
+  | TyPrim p ixs => rho p (expsAsSub ixs)
+  | TyAll    s t => fun x y => forall rho', ES rho' -> rho' >> rho -> semTy rho' x y
+  | TyExists s t => difclo (fun x y => exists rho', ES rho' /\ rho' >> rho /\ semTy rho' x y)
+  end.
+
+Implicit Arguments semTy [D].  
+
+(*Notation "rho |= x == y :> t" := (semTy (t:=t) rho x y) (at level 67, x at level 67, y at level 67).*)
+
+Fixpoint semCtxt D (rho: RelEnv D) (G:Ctxt D) : relation (interpCtxt G) :=
+  if G is t::G then fun eta1 eta2 => semTy rho t eta1.1 eta2.1 /\ semCtxt rho eta1.2 eta2.2
+  else fun _ _ => True.
+
+(*---------------------------------------------------------------------------
+   Unfortunately we need casts just to state the semSubst and semEquiv lemmas. 
+   "up" sends a value from |t| to |apSubTy S t|
+   "dn" sends a value from |apSubTy S t| to |t|
+   We have various lemmas connecting these.
+   ---------------------------------------------------------------------------*)
+Section UpDn. 
+
+  Variables D D' : IxCtxt sig.
+  Variables S : Sub D D'.
+  Variables t t1 t2 : Ty D.
+  Variables E : equivTy A t1 t2.
+
+  Definition up t x := x :? interpSubst t S.
+  Definition dn t x := x :? sym_equal (interpSubst t S).
+  Definition rt x := x :? interpEquiv E.
+
+  Lemma dnup (x: |t|) : dn (up x) = x.
+  Proof. by rewrite /up/dn cast_coalesce cast_id. Qed. 
+
+  Lemma updn (x: |apSubTy S t|) : up (dn x) = x.
+  Proof. by rewrite /up/dn cast_coalesce cast_id. Qed. 
+End UpDn.
+
+Section UpDnProps.
+
+  Variables D D' : IxCtxt sig.
+  Variables S : Sub D D'.
+  Variables t t1 t2 t1' t2' : Ty D.
+
+  Lemma upApp (f: |TyArr t1 t2|) (x: |t1|) : up S (f x) = (up _ f) (up S x). 
+  Proof. rewrite /up. apply cast_app. Qed. 
+
+  Lemma upFst (p: |TyProd t1 t2|) : (up _ p).1 = (up S p.1).
+  Proof. rewrite /up. apply (cast_fst (interpSubst t1 S) (interpSubst t2 S)). Qed. 
+
+  Lemma upSnd (p: |TyProd t1 t2|) : (up _ p).2 = (up S p.2).
+  Proof. rewrite /up. apply (cast_snd (interpSubst t1 S) (interpSubst t2 S)). Qed. 
+
+  Lemma upInl (x: |t1|) : up (t:=TySum t1 t2) S (inl _ x) = inl _ (up (t:=t1) S x).
+  Proof.  
+  rewrite /up. apply (cast_inl (interpSubst t1 S) (interpSubst t2 S)). 
+  Qed. 
+
+  Lemma upInr (x: |t2|) : up (t:=TySum t1 t2) S (inr _ x) = inr _ (up (t:=t2) S x).
+  Proof.  
+  rewrite /up. apply (cast_inr (interpSubst t1 S) (interpSubst t2 S)). 
+  Qed. 
+
+  Lemma upSpec s (ty: Ty (s::D)) (x: | TyAll ty|): up S x = up (liftSub _ S) x.
+  Proof. rewrite /up. by apply cast_UIP. Qed. 
+
+  Lemma upInst s (ty: Ty (s::D)) (x: | TyExists ty|): up S x = up (liftSub _ S) x.
+  Proof. rewrite /up. by apply cast_UIP. Qed. 
+
+End UpDnProps.
+
+
+Lemma invEnvK D (R: RelEnv D) : invEnv (invEnv R) = R. 
+Proof. 
+apply functional_extensionality_dep => p.  
+apply functional_extensionality => z.
+apply functional_extensionality => z'. 
+by apply functional_extensionality. 
+Qed. 
+
+Lemma invExt s D (rho': RelEnv (s::D)) (rho: RelEnv D) :
+  rho' >> invEnv rho -> invEnv rho' >> rho. 
+Proof. rewrite /ext. move => H.  
+apply functional_extensionality_dep => p. 
+apply functional_extensionality => S. 
+apply functional_extensionality => z. 
+apply functional_extensionality => z'.
+have H': EcS rho' (pi D s) S z' z = invEnv rho S z' z. by rewrite H. 
+rewrite /invEnv in H'. by rewrite -H'. 
+Qed. 
+
+Variable CLOSED: ClosedRelEnvSet A ES. 
+
+Lemma semInv : forall D (t : Ty D) rho x x', semTy rho t x x' -> semTy (invEnv rho) t x' x. 
+Proof.
+  induction t => /= rho x x' xx'. 
+  (* TyUnit *)
+  done. 
+
+  (* TyProd *)
+  split; firstorder. 
+
+  (* TySum *)
+  destruct x'; destruct x; firstorder. 
+
+  (* TyArr *)
+  move => y y' yy'. specialize (IHt1 _ _ _ yy'). 
+  rewrite invEnvK in IHt1. specialize (xx' _ _ IHt1). 
+  by apply (IHt2 _ _ _ xx'). 
+
+  (* TyPrim *)
+  rewrite /invEnv. apply xx'. 
+  
+  (* TyAll *)  
+  move => rho' ESrho' EXT. 
+  specialize (IHt (invEnv rho') x x'). rewrite invEnvK in IHt. apply IHt.
+  apply xx'. by apply (closedWrtInv CLOSED). by apply: invExt EXT. 
+
+  (* TyExists *)
+  induction xx'.
+   (* base *)
+   apply difclo_base. 
+    destruct H as [rho' [ESrho' [EXT H]]]. 
+    exists (invEnv rho'). split. by apply (closedWrtInv CLOSED). 
+    split. apply invExt. rewrite invEnvK. apply EXT. apply IHt. apply H. 
+   (* step *)
+   eapply difclo_step; eassumption.
+Qed. 
+
+Lemma semTyCast D1 D2 (t1: Ty D1) (t2: Ty D2) rho (v1 v2: |t1|) (p1 p2 p3 p4: (|t1|) = (|t2|) ) : 
+  semTy rho t2 (v1 :? p1) (v2 :? p2) ->
+  semTy rho t2 (v1 :? p3) (v2 :? p4).
+Proof.   
+move => H.
+by rewrite (cast_UIP v1 _ p1) (cast_UIP v2 _ p2). 
+Qed. 
+
+(* This is lemma 2, part 1 *)
+Lemma semEquiv D (t1 t2: Ty D) (E: equivTy A t1 t2) : forall (rho: RelEnv D) (v v':interpTy t1),
+  ES rho -> 
+  (semTy rho t1 v v' <->
+  semTy rho t2 (rt E v) (rt E v')). 
+Proof. 
+(* Not sure why this needs generalizing. But the induction won't go through otherwise. *)
+rewrite /rt. move: (interpEquiv E).
+induction E => pf rho v v' ESrho. 
+(* EquivTyRefl *)
+by rewrite 2!cast_id. 
+(* EquivTySym *)
+rewrite (IHE CLOSED (sym_equal pf)) => //. rewrite cast_coalesce => //. 
+rewrite cast_id. rewrite cast_coalesce. by rewrite cast_id. 
+(* EquivTyTrans *)
+rewrite (IHE1 CLOSED (interpEquiv E1)) => //.
+rewrite (IHE2 CLOSED (interpEquiv E2)) => //. 
+rewrite 2!cast_coalesce.  
+split => H. apply (semTyCast _ _ H). apply (semTyCast _ _ H). 
+(* EquivTyProd *)
+simpl. rewrite !(cast_fst (interpEquiv E1) _). 
+rewrite !(cast_snd _ (interpEquiv E2)). 
+rewrite -(IHE1 _ (interpEquiv E1)) => //. rewrite -(IHE2 _ (interpEquiv E2)) => //. 
+apply (interpEquiv E1). apply (interpEquiv E1). apply (interpEquiv E2). apply (interpEquiv E2). 
+(* EquivTySum *)
+destruct v. 
+destruct v'.
++ simpl. by rewrite !(cast_inl (interpEquiv E1) (interpEquiv E2)) -IHE1. 
++ simpl. by rewrite !(cast_inr (interpEquiv E1) (interpEquiv E2))
+        !(cast_inl (interpEquiv E1) (interpEquiv E2)). 
+destruct v'. 
++ simpl. by rewrite !(cast_inr (interpEquiv E1) (interpEquiv E2))
+        !(cast_inl (interpEquiv E1) (interpEquiv E2)). 
++ simpl. by rewrite !(cast_inr (interpEquiv E1) (interpEquiv E2)) -IHE2. 
+(* EquivTyArr *)
+have eq1:=interpEquiv E1. have eq2:=interpEquiv E2.
+simpl. 
+split => H x x' xx'.
++ rewrite 2!cast_appFun. 
+  rewrite -IHE2 => //. 
+  apply H. 
+  rewrite (IHE1 _ eq1) => //. 
+  rewrite !cast_coalesce. rewrite !cast_id. apply xx' => //. 
++ rewrite (IHE2 _ eq2) => //. 
+  specialize (H (x :? eq1) (x' :? eq1)). 
+  rewrite 2!(cast_app eq1 eq2). apply H. 
+  rewrite -IHE1 => //. 
+(* EquivTyPrim *)
+simpl.
+rewrite !cast_id. 
+have GE := goodEnvs CLOSED ESrho.  rewrite /GoodRelEnv in GE. 
+by rewrite (GE op es es' H). 
+(* EquivTyAll *)
+simpl. split. 
+move => H rho' ESrho' EXTrho'. rewrite -IHE. apply H => //. apply CLOSED. apply ESrho'. 
+move => H rho' ESrho' EXTrho'. rewrite IHE. apply H => //. apply CLOSED. apply ESrho'. 
+(* EquivTyExists *)
+simpl. symmetry. apply difclo_cast3. split.
+move => [rho' [ESrho' [EXTrho' H]]]. exists rho'. rewrite IHE. split. done. split. done. apply H. apply CLOSED. apply ESrho'. 
+move => [rho' [ESrho' [EXTrho' H]]]. exists rho'. rewrite -IHE. split; done. apply CLOSED => //. apply ESrho'.
+Qed.
+
+Lemma sem_difunctional : 
+  (forall D (psi: RelEnv D) p exps, ES psi -> difunctional (psi p exps)) ->
+  forall D (t: Ty D) (psi: RelEnv D), ES psi -> difunctional (semTy psi t).
+Proof.
+  move => DIF. 
+  induction t => /= rho inES. 
+  
+  (* TyUnit *)
+  by intuition. 
+
+  (* TyProd *)
+  specialize (IHt1 rho inES). specialize (IHt2 rho inES). by apply: prod_difunctional.  
+
+  (* TySum *)
+  specialize (IHt1 rho inES). specialize (IHt2 rho inES). by apply: sum_difunctional.
+
+  (* TyArrow *)
+  specialize (IHt1 rho inES). specialize (IHt2 rho inES). by apply: arrow_difunctional. 
+
+  (* TyBase *)
+  apply DIF. apply inES.
+
+  (* For all *)
+  intros x x' y y' xy x'y' xy'.
+  intros psi' ESpsi' ext.
+  assert (xy0 := xy psi' ESpsi' ext).
+  assert (x'y'0 := x'y' psi' ESpsi' ext).
+  assert (xy'0 := xy' psi' ESpsi' ext).
+  by apply (IHt psi' ESpsi' x x' y y' xy0 x'y'0 xy'0). 
+
+  (* Exists *)
+  apply: difclo_difunctional.
+Qed. 
+
+(* This is lemma 2, part 2 *)
+Lemma semSubst D (t: Ty D) : forall D' (S:Sub D D') rho (ESrho: ES rho) v v',
+  semTy rho (apSubTy S t) (up S v) (up S v')
+  <->
+  semTy (EcS rho S) t v v'.
+Proof. induction t => /= D' S rho ESrho v v'.
+
+(* TyUnit *)
+by reflexivity. 
+
+(* TyProd *)
+by rewrite -(IHt1 _ S rho ESrho) -(IHt2 _ S rho ESrho) 2!upFst 2!upSnd. 
+
+(* TySum *)
+specialize (IHt1 D' S rho ESrho). specialize (IHt2 D' S rho ESrho). 
+set x := up S _. simpl in x.
+case E: x => [x1 | x2]. 
+* set x' := up S _. simpl in x'. 
+  case E': x' => [x'1 | x'2].
+  + case E'': v => [v1 | v2]. 
+    - rewrite /x E'' upInl in E. inversion E. clear E. 
+      case E''': v' => [v1' | v2']. 
+        rewrite -IHt1.
+        rewrite /x' E''' upInl in E'. inversion E'. clear E'. 
+        by rewrite H0 H1.
+        rewrite /x' E''' upInr in E'. inversion E'. 
+    - rewrite /x E'' upInr in E. inversion E.
+  + case E'': v => [v1 | v2].  
+    - rewrite /x E'' upInl in E. inversion E. clear E. 
+      case E''': v' => [v1' | v2']. 
+      rewrite -IHt1. 
+      rewrite /x' E''' upInl in E'. inversion E'. 
+      done. 
+    - rewrite /x E'' upInr in E. inversion E. 
+* set x' := up S _. simpl in x'. 
+  case E': x' => [x'1 | x'2].
+  + case E'': v => [v1 | v2]. 
+    - rewrite /x E'' upInl in E. inversion E. 
+    - rewrite /x E'' upInr in E. inversion E. clear E. 
+      case E''': v' => [v1' | v2']. 
+        done.         
+        rewrite -IHt2.
+        rewrite /x' E''' upInr in E'. inversion E'. 
+  + case E'': v => [v1 | v2]. 
+    - rewrite /x E'' upInl in E. inversion E. 
+    - rewrite /x E'' upInr in E. inversion E. clear E. rewrite H0. 
+      case E''': v' => [v1' | v2']. 
+      rewrite /x' E''' upInl in E'. inversion E'. 
+      rewrite /x' E''' upInr in E'. inversion E'. clear E'. 
+      rewrite -IHt2. by rewrite H0 H1. 
+
+(* TyArr *)
+specialize (IHt1 D' S rho ESrho). 
+specialize (IHt2 D' S rho ESrho). 
+split. 
++ move => H x x' xx'. destruct (IHt1 x x') as [_ IHb]. 
+  specialize (IHb xx'). 
+  specialize (H _ _ IHb). 
+  rewrite -2!upApp in H.   
+  by rewrite ->IHt2 in H. 
++ move => H x x' xx'. 
+  destruct (IHt1 (dn x) (dn x')) as [IHa _]. 
+  rewrite !updn in IHa. 
+  specialize (IHa xx'). 
+  specialize (H _ _ IHa). 
+  destruct (IHt2 (v (dn x)) (v' (dn x'))) as [_ IHd]. 
+  specialize (IHd H). by rewrite !upApp!updn in IHd. 
+
+(* TyPrim *)
+rewrite /EcS/up/=.
+rewrite ScExpsAsSub. by rewrite cast_UIP cast_id cast_UIP cast_id. 
+
+(* TyAll *)
+specialize (IHt _ (liftSub _ S)).
+split => H rho' ESrho' EXT. 
+  (* For this case we need second closure property of environments *)
++ have CL2 := closedWrtLift CLOSED ESrho' ESrho EXT. 
+  destruct CL2 as [rho0 [H2 [H3 H4]]]. 
+  destruct (IHt rho0 H2 v v') as [IH1 _].
+  rewrite -!upSpec in IH1. 
+  specialize (H _ H2 H4). 
+  rewrite H3 in IH1. apply IH1. 
+  by apply H. 
+
+  (* This time we need first closure property of environments,
+     together with simple properties of pi and lifting *)
++ specialize (IHt rho' ESrho' v v'). 
+  rewrite -!upSpec in IHt. apply IHt. apply H. 
+  apply (closedWrtSubst CLOSED (liftSub s S) ESrho').    
+  rewrite /ext in EXT. rewrite -EXT.  
+  apply functional_extensionality_dep => p. 
+  apply functional_extensionality => S'.
+  rewrite /EcS 2!ScS_assoc. 
+  by rewrite liftPi.  
+
+(* TyExists *)
+unfold up.
+apply difclo_cast3.
+split => [[rho' [H1 [H2 H3]]] | [rho1 [H1 [H2 H3]]]]. 
++ exists (EcS rho' (liftSub _ S)).
+  split. by apply (closedWrtSubst CLOSED). 
+  split. rewrite /ext. rewrite -H2. 
+  apply functional_extensionality_dep => p. 
+  apply functional_extensionality => S'. 
+  rewrite /EcS 2!ScS_assoc.
+  by rewrite liftPi.
+
+  specialize (IHt _ (liftSub s S) rho' H1 x y). rewrite -IHt.
+  rewrite -2!upInst. apply H3. 
+
++ have CL1 := closedWrtLift CLOSED.   
+  specialize (CL1 _ _ s S rho1 H1 _ ESrho H2). 
+  destruct CL1 as [rho0 [H4 [H5 H6]]]. 
+  exists rho0.  
+  split => //. 
+  split => //. 
+  specialize (IHt _ (liftSub s S) _ H4 x y). 
+  change (x :? interpSubst (TyExists t) S) with (@up D D' S (TyExists t) x).
+  change (y :? interpSubst (TyExists t) S) with (@up D D' S (TyExists t) y).
+  rewrite 2!upInst.
+  rewrite IHt {IHt}.
+  rewrite H5. apply H3. 
+Qed.
+
+Lemma AbstractionVar D (G: Ctxt D) (t: Ty D) (v: TmVar G t) (rho: RelEnv D) eta1 eta2:
+  semCtxt rho eta1 eta2 -> semTy rho t (interpTmVar v eta1) (interpTmVar v eta2). 
+Proof. induction v => /= H. 
++ apply H. + apply IHv. apply H. 
+Qed. 
+
+Lemma castConsCtxt D D' (t: Ty D) (G: Ctxt D) (S: Sub D D') (v:|t|) (eta: interpCtxt G) : 
+  ((v, eta) :? (interpSubCtxt (t :: G) S)) = 
+  (v :? interpSubst t S, eta :? interpSubCtxt G S). 
+Proof.
+apply (cast_pair (interpSubst t S) (interpSubCtxt G S)).
+Qed.
+
+
+(* This is lemma 4 *)
+Lemma semSubstCtxt D (G: Ctxt D) : forall D' (S:Sub D D') rho (ESrho: ES rho) eta eta',
+  semCtxt rho (eta :? interpSubCtxt G S) (eta' :? interpSubCtxt G S)
+  <->
+  semCtxt (EcS rho S) eta eta'.  
+Proof. induction G => //.  
+move => D' S rho ESrho [v eta] [v' eta']. 
+fold interpCtxt in *.
+specialize (IHG _ S _ ESrho eta eta').
+simpl semCtxt.  
+rewrite -IHG. 
+rewrite !castConsCtxt. simpl. split. 
+move => [H1 H2]. 
+split => //. 
+apply semSubst => //. 
+move => [H1 H2]. 
+split => //. 
+apply semSubst => //. 
+Qed.  
+
+Variable DIF : forall D (psi: RelEnv D) p exps, ES psi -> difunctional (psi p exps).
+
+
+(* Theorem 1 *)
+Theorem Abstraction D (G: Ctxt D) (t: Ty D) (M: Tm A G t) (rho: RelEnv D) eta1 eta2:
+  ES rho -> 
+  semCtxt rho eta1 eta2 -> semTy rho t (interpTm M eta1) (interpTm M eta2). 
+Proof. induction M => /= ESrho H. 
+(* VAR *)
+apply AbstractionVar => //. 
+(* TYEQ *)
+apply semEquiv => //. apply IHM => //. 
+(* UNIT *)
+done. 
+(* PAIR *)
+split; [apply IHM1 => // | apply IHM2 => //].
+(* PROJ1 *)
+apply IHM => //.
+(* PROJ2 *)
+apply IHM => //. 
+(* INL *)
+apply IHM => //. 
+(* INR *)
+apply IHM => //. 
+(* CASE *)
+simpl in IHM1.
+specialize (IHM1 rho eta1 eta2 ESrho H). 
+case E1: (interpTm M1 eta1) => [a | a]. 
+case E2: (interpTm M1 eta2) => [b | b]. 
++ rewrite E1 E2 in IHM1. by apply IHM2 => //. 
++ by rewrite E1 E2 in IHM1. 
+case E2: (interpTm M1 eta2) => [b | b]. 
++ by rewrite E1 E2 in IHM1. 
++ rewrite E1 E2 in IHM1. by apply IHM3 => //. 
+(* ABS *)
+move => x x' xx'. apply IHM => //.   
+(* APP *)
+apply IHM1 => //. apply IHM2 => //. 
+(* UNIVABS *)
+move => rho' ESrho' EXT.
+apply IHM => //. rewrite /ext in EXT. rewrite -EXT in H.
+apply semSubstCtxt => //. 
+(* UNIVAPP *)
+specialize (IHM rho _ _ ESrho H). simpl in IHM.
+have ESrho': ES (EcS rho (consSub e (idSub D))) by apply (closedWrtSubst CLOSED) => //. 
+have EXTrho': EcS rho (consSub e (idSub D)) >> rho.
+rewrite /ext/EcS. apply functional_extensionality_dep => p.  
+apply functional_extensionality => ixs. rewrite ScS_assoc. by rewrite consPi idScS. 
+specialize (IHM _ ESrho' EXTrho'). have SS := proj2 (semSubst _ _ _ _) IHM. 
+specialize (SS ESrho).
+apply: semTyCast SS.  
+(* EXPACK *)
+apply difclo_base.
+specialize (IHM rho eta1 eta2 ESrho H). exists (EcS rho (consSub e (idSub D))). 
+split. apply (closedWrtSubst CLOSED) => //. 
+split. rewrite /ext/EcS. 
+apply functional_extensionality_dep => p.  
+apply functional_extensionality => ixs. rewrite ScS_assoc. by rewrite consPi idScS. 
+have SS := (semSubst (consSub e (idSub D)) _ (interpTm M eta1 :? _) (interpTm M eta2 :? _) (t:=t) (rho:=rho)).
+destruct (SS ESrho (sym_equal (interpSubst _ _)) (sym_equal (interpSubst _ _))) as [SS1 _].
+clear SS. rewrite /up !cast_coalesce !cast_id in SS1. specialize (SS1 IHM).
+apply: semTyCast SS1. 
+(* EXUNPACK *)
+specialize (IHM1 rho eta1 eta2 ESrho H). simpl in IHM1. 
+induction IHM1.
+ (* base *)
+ destruct H0 as [rho' [ESrho' [EXTrho' IHM1]]].
+ simpl in IHM2.  
+ specialize (IHM2 rho' (x, eta1 :? interpSubCtxt G (pi D s))
+                       (y, eta2 :? interpSubCtxt G (pi D s)) ESrho'). 
+ simpl in IHM2. 
+ rewrite /ext in EXTrho'. 
+ rewrite -EXTrho'. rewrite -EXTrho' in H. 
+ have H2: semCtxt rho' (eta1 :? interpSubCtxt G (pi D s)) (eta2 :? interpSubCtxt G (pi D s)).
+ by apply semSubstCtxt => //. 
+ rewrite !cast_id. specialize (IHM2 (conj IHM1 H2)). 
+ have SS := (@semSubst _ t' _ (pi D s) rho' ESrho'). rewrite /up in SS. 
+ apply SS. rewrite !cast_coalesce !cast_id. apply IHM2. 
+ (* step *)
+ eapply sem_difunctional; eassumption.
+Qed. 
+
+(*---------------------------------------------------------------------------
+   Models of equational theory
+   ---------------------------------------------------------------------------*)
+Fixpoint interpSeq X (interp: X -> Type) (xs: seq X): Type :=
+  if xs is x::xs then (interp x * interpSeq interp xs)%type
+  else unit.
+
+(* Interpretation of sorts and index operations *)
+Structure Interpretation := mkIntepretation {
+  (* Carrier for each sort *)
+  interpSrt : Srt sig -> Type; 
+
+  (* Function for each index operation *)
+  interpOp : forall p, interpSeq interpSrt (opArity p).1 -> interpSrt (opArity p).2  
+}.
+
+Implicit Arguments interpOp [].
+
+Fixpoint interpVar I D s (v: Var D s) : interpSeq (interpSrt I) D -> interpSrt I s :=
+  match v with 
+  | VarZ _ _     => fun env => env.1
+  | VarS _ _ _ v => fun env => interpVar v env.2
+  end.
+
+(* Interpret an index expression compositionally *)
+Fixpoint interpExp I D s (e: Exp D s) : interpSeq (interpSrt I) D -> interpSrt I s :=
+  match e with
+  | VarAsExp _ v => fun env => interpVar v env
+  | AppCon op es => fun env => interpOp I op (interpExps es env)
+  end
+
+with interpExps I D ss (es: Exps D ss) (env: interpSeq (interpSrt I) D)
+  : interpSeq (interpSrt I) ss :=
+  if es is Cons _ _ ix ixs then (interpExp ix env, interpExps ixs env) else tt.
+
+Definition interpAx I (A: Ax sig) := 
+  let: mkAx D s lhs rhs := A in
+  forall env: interpSeq (interpSrt I) D, interpExp lhs env = interpExp rhs env.
+
+Fixpoint interpAxs I (As: seq (Ax sig)) :=
+  if As is A::As then interpAx I A /\ interpAxs I As else True.
+
+(* A model is an interpretation together with a proof that the axioms are satisfied *)
+Structure Model := mkModel {
+  I :> Interpretation;
+  soundness: interpAxs I A
+}.
+
+Fixpoint apArgs (M1 M2: Model) arity (f:forall s, interpSrt M1 s -> interpSrt M2 s) :
+  interpSeq (interpSrt M1) arity -> interpSeq (interpSrt M2) arity :=
+  if arity is s::ss
+  then fun args => (f s args.1, apArgs f args.2) 
+  else fun args => tt.
+ 
+Structure Homomorphism (M1 M2: Model) := mkHom {
+  hom:> forall s: Srt sig, interpSrt M1 s -> interpSrt M2 s;
+  preserves: forall p xs, hom (interpOp M1 p xs) = interpOp M2 p (apArgs hom xs)
+}.
+
+(* TODO: free models *)
+
+End Sem.
